dataplane/Timely_Infrastructure.thy
@@ -2136,4 +2136,193 @@ lemma in_cimage_cset_from_list[simp]:
   apply (auto simp flip: cin.rep_eq)
   done 
 
+
+
+
+lemma remove_last_not_Nil:
+  "x \<notin> set xs \<Longrightarrow> remove_last x xs = xs"
+  apply (induct xs rule: rev_induct)
+   apply clarsimp
+  subgoal for x' xs'
+    apply simp
+    apply (cases xs'; clarsimp)
+    done
+  done
+
+lemma remove_last_in_set_Cons:
+  "x \<in> set xs \<Longrightarrow> remove_last x (x' # xs) = x' # remove_last x xs"
+  apply (induct xs rule: rev_induct)
+   apply simp
+  subgoal for x xs'
+    apply (cases xs')
+    subgoal
+      by simp
+    subgoal
+      by fastforce
+    done
+  done
+
+lemma remove_last_not_in_set_Cons:
+  "x \<notin> set xs \<Longrightarrow> remove_last x (x # xs) = xs"
+  apply (induct xs rule: rev_induct)
+   apply simp
+  subgoal for x xs'
+    apply (cases xs')
+    subgoal
+      by simp
+    subgoal
+      by fastforce
+    done
+  done
+
+lemma remove_last_append_if:
+  "remove_last x (xs @ ys) = (if x \<in> set ys then xs @ remove_last x ys else remove_last x xs @ ys)"
+  apply (induct xs arbitrary: ys rule: rev_induct)
+   apply (clarsimp simp add: remove_last_not_Nil split: if_splits)
+  subgoal premises prems for x' xs ys
+    apply auto
+    subgoal
+      apply (subst prems(1))
+      apply (simp del: remove_last.simps)
+      apply (subst remove_last_in_set_Cons)
+       apply auto
+      done
+    subgoal
+      apply (subst prems(1))
+      apply (clarsimp simp del: remove_last.simps)
+      apply (intro conjI impI)
+      subgoal
+      apply (subst remove_last_not_in_set_Cons)
+        using prems(1) apply auto
+        done
+      subgoal
+        apply (subst prems(1))
+        apply auto
+        done
+      done
+    done
+  done
+
+
+lemma remove_last_append_singleton[simp]:
+  "remove_last x (xs @ [x]) = xs"
+  apply (induct x "xs @ [x]" rule: remove_last.induct)
+   apply simp_all
+  apply (metis append.right_neutral distinct.simps(2) distinct_singleton list.set_intros(1) remove_last_append_if remove_last_not_in_set_Cons)
+  done
+
+lemma remove_last_append_diff_singleton:
+  "x \<noteq> y \<Longrightarrow> remove_last y (xs @ [x]) = remove_last y xs @ [x]"
+  apply (induct y "xs @ [x]" rule: remove_last.induct)
+   apply simp_all
+  apply (subst remove_last_append_if)
+  apply simp
+  done
+
+lemma remove_last_Cons_if:
+  "remove_last a (a # xs) = (if a \<in> set xs then a # remove_last a xs else xs)"
+  apply (induct xs rule: rev_induct)
+  subgoal
+   apply (simp del: remove_last.simps)
+    apply (subst remove_last.simps)
+   apply (simp del: remove_last.simps)
+    done
+  subgoal for x xs'
+   apply (auto simp del: remove_last.simps split: if_splits)
+    subgoal
+    apply (subst remove_last.simps)
+   apply (clarsimp simp del: remove_last.simps split: if_splits)
+      done
+    subgoal
+    apply (subst remove_last.simps)
+   apply (clarsimp simp del: remove_last.simps simp add: remove_last_append_diff_singleton split: if_splits)
+      done
+    subgoal
+    apply (subst remove_last.simps)
+   apply (clarsimp simp del: remove_last.simps split: if_splits)
+      done
+    subgoal
+    apply (subst remove_last.simps)
+   apply (clarsimp simp del: remove_last.simps simp add: remove_last_append_diff_singleton split: if_splits)
+      done
+    done
+  done
+
+lemma remove_last_append_in_set:
+  "a \<in> set ys \<Longrightarrow>
+   remove_last a (xs @ ys) = xs @ remove_last a ys"
+  by (simp add: remove_last_append_if)
+
+lemma remove_last_append_not_in_set:
+  "a \<notin> set ys \<Longrightarrow>
+   remove_last a (xs @ ys) = remove_last a xs @  ys"
+  by (simp add: remove_last_append_if)
+
+lemma list_diff_same_sufix:
+  "mset ys = mset zs \<Longrightarrow>
+   list_diff (xs @ zs) ys = xs"
+  apply (induct "xs @ zs" ys arbitrary: xs zs rule: list_diff.induct)
+  apply auto
+  subgoal premises prems for x xs xs' zs
+    using prems(2) apply -
+    apply (drule sym)
+    using prems(1) 
+    apply (metis mset_remove_last remove1_mset_add_mset_If remove_last_append_if set_mset_mset union_single_eq_member)
+    done
+  done
+
+lemma list_diff_append[simp]:
+  "list_diff zs (xs @ ys) = list_diff (list_diff zs xs) ys"
+  apply (induct xs arbitrary: zs ys)
+   apply simp_all
+  done
+
+lemma list_diff_append_append:
+  "mset zs1 = mset zs2 \<Longrightarrow>
+   list_diff (xs @ zs1) (zs2 @ ys) = list_diff xs ys"
+  apply simp
+  apply (subst list_diff_same_sufix)
+   apply auto
+  done
+
+lemma in_set_list_diffD:
+  "x \<in> set (list_diff xs ys) \<Longrightarrow> x \<in> set xs"
+  by (induct xs ys arbitrary: xs rule: list_diff.induct)
+    (auto dest: set_remove_lastD)
+
+
+lemma not_in_set_list_diff_same_count:
+  "count (mset xs) y = count (mset ys) y \<Longrightarrow>
+   y \<in> set (list_diff xs ys) \<Longrightarrow> False"
+  apply (induct xs ys arbitrary: xs rule: list_diff.induct)
+   apply clarsimp
+  apply force
+  done
+
+lemma in_set_list_diffI[intro]:
+  "x \<in> set xs \<Longrightarrow> x \<notin> set ys \<Longrightarrow> x \<in> set (list_diff xs ys)"
+    apply (induct xs ys arbitrary: xs rule: list_diff.induct)
+  apply clarsimp+
+  subgoal premises prems for y xs ys
+    apply (rule prems(1))
+    using prems(2-) apply -
+    apply (metis (no_types, lifting) in_set_conv_decomp remove_last_append_in_set remove_last_append_not_in_set remove_last_in_set_Cons set_ConsD)
+    done
+  done
+
+
+lemma set_list_diff_filter[simp]:
+  "set (list_diff xs (filter P xs)) = {x \<in> set xs. \<not> P x}"
+  apply (induct "filter P xs" arbitrary: xs rule: rev_induct)
+   apply (simp add: List.empty_filter_conv basic_trans_rules(24) subsetI)
+  subgoal premises prems for x xs' xs''
+    apply (auto dest: in_set_list_diffD)
+    subgoal
+      apply (drule not_in_set_list_diff_same_count[rotated])
+       apply auto
+      done
+    done
+  done
+
+
 end
